Term/WithArity/AMonAlg.v
@@ -4,8 +4,9 @@ See the COPYRIGHTS and LICENSE files.
 
 - Adam Koprowski and Hans Zantema, 2007-03
 
-  This file contains a definition of weakly monotone algebra and extended monotone
-algebra and some results concerning them, based on:
+  This file contains a definition of weakly monotone algebra and
+  extended monotone algebra and some results concerning them, based
+  on:
 
 References:
 -  J. Endrullis, J. Waldmann and H. Zantema, "Matrix Interpretations for Proving
@@ -18,6 +19,7 @@ Require Export AWFMInterpretation.
 (***********************************************************************)
 (** * Module type specifying a weakly monotone algebra.                *)
 (***********************************************************************)
+
 Module Type MonotoneAlgebraType.
 
   Parameter Sig : Signature.
@@ -54,7 +56,8 @@ Module Type MonotoneAlgebraType.
   Notation term := (term Sig).
 
   Parameters (succ' : relation term) (succeq' : relation term).
-  Parameters (succ'_sub : succ' << IR_succ) (succeq'_sub : succeq' << IR_succeq).
+  Parameters (succ'_sub : succ' << IR_succ)
+    (succeq'_sub : succeq' << IR_succeq).
   Parameters (succ'_dec : rel_dec succ') (succeq'_dec : rel_dec succeq').
 
 End MonotoneAlgebraType.
@@ -62,13 +65,14 @@ End MonotoneAlgebraType.
 (***********************************************************************)
 (** * Module type specifying an extended weakly monotone algebra.      *)
 (***********************************************************************)
+
 Module Type ExtendedMonotoneAlgebraType.
 
   Declare Module MA : MonotoneAlgebraType.
   Export MA.
 
-  (** Extended monotone algebra is a wekaly monotone algebra in which every operation
-      is monotone with respect to [succ] *)
+  (** Extended monotone algebra is a wekaly monotone algebra in which
+  every operation is monotone with respect to [succ] *)
   Parameter monotone_succ : monotone I succ.
 
 End ExtendedMonotoneAlgebraType.
@@ -76,6 +80,7 @@ End ExtendedMonotoneAlgebraType.
 (***********************************************************************)
 (** * Functor with a theory of weakly monotone algebras                *)
 (***********************************************************************)
+
 Module MonotoneAlgebraResults (MA : MonotoneAlgebraType).
 
   Export MA.
@@ -97,7 +102,8 @@ Module MonotoneAlgebraResults (MA : MonotoneAlgebraType).
     exists (term_int val y). split; auto.
   Qed.
 
-  Lemma IR_rewrite_ordering : forall succ, monotone I succ -> rewrite_ordering (IR I succ).
+  Lemma IR_rewrite_ordering : forall succ,
+    monotone I succ -> rewrite_ordering (IR I succ).
 
   Proof.
     split.
@@ -116,13 +122,14 @@ Module MonotoneAlgebraResults (MA : MonotoneAlgebraType).
 
 (**********************************************************************)
 (** top termination (for DP setting) criterion with monotone algebras *)
+
   Section TopTermination.
 
     Variable R E : rules.
 
     Lemma ma_compat_hd_red_mod : 
-      compatible IR_succ R ->
-      compatible IR_succeq E ->
+      compat IR_succ R ->
+      compat IR_succeq E ->
       WF (hd_red_mod E R).
 
     Proof.
@@ -141,6 +148,7 @@ End MonotoneAlgebraResults.
 (***********************************************************************)
 (** * Functor with a theory of extended monotone algebras              *)
 (***********************************************************************)
+
 Module ExtendedMonotoneAlgebraResults (EMA : ExtendedMonotoneAlgebraType).
 
   Module MAR := MonotoneAlgebraResults EMA.MA.
@@ -158,14 +166,15 @@ Module ExtendedMonotoneAlgebraResults (EMA : ExtendedMonotoneAlgebraType).
 
 (**********************************************************)
 (** relative termination criterion with monotone algebras *)
+
   Section RelativeTermination.
 
     Variable R E : rules.
 
     (* Termination in one go *)
     Lemma ma_compat_red_mod : 
-      compatible IR_succ R ->
-      compatible IR_succeq E ->
+      compat IR_succ R ->
+      compat IR_succeq E ->
       WF (red_mod E R).
 
     Proof.
@@ -182,6 +191,7 @@ Module ExtendedMonotoneAlgebraResults (EMA : ExtendedMonotoneAlgebraType).
 (**********************************************************)
 (** results and tactics for proving relative termination 
     of concrete examples. *)
+
   Section RelativeTerminationCriterion.
 
     Definition rule_partition R (R_dec : rel_dec R) (r : rule Sig) := 
@@ -194,7 +204,8 @@ Module ExtendedMonotoneAlgebraResults (EMA : ExtendedMonotoneAlgebraType).
 
     Proof.
       intros. unfold rule_partition in H.
-      set (w := partition_left (fun r => partition_by_rel R_dec (lhs r, rhs r))). simpl in w.
+      set (w := partition_left
+        (fun r => partition_by_rel R_dec (lhs r, rhs r))). simpl in w.
       change l with (lhs (mkRule l r)). change r with (rhs (mkRule l r)).
       apply w with rs. assumption.
     Qed.
@@ -221,9 +232,9 @@ Module ExtendedMonotoneAlgebraResults (EMA : ExtendedMonotoneAlgebraType).
       apply red_union.
     Qed.
 
-    Lemma partition_compatible : forall R succ succ'
+    Lemma partition_compat : forall R succ succ'
       (succ'_dec : rel_dec succ'), succ' << succ ->
-      compatible succ (fst (partition (rule_partition succ'_dec) R)).
+      compat succ (fst (partition (rule_partition succ'_dec) R)).
 
     Proof.
       clear R E. intros R ord ord' ord'_dec ord'_sub l r lr.
@@ -254,12 +265,12 @@ Module ExtendedMonotoneAlgebraResults (EMA : ExtendedMonotoneAlgebraType).
       unfold red_mod. comp. 
       apply incl_rtc. apply red_union_inv. apply red_union_inv.
       apply ma_compat_red_mod; trivial.
-      apply compatible_app.
-      unfold Rgt, R_gt, part_succ. apply partition_compatible. exact succ'_sub.
-      unfold Egt, E_gt, part_succ. apply partition_compatible. exact succ'_sub.
-      apply compatible_app.
-      unfold Rge, R_ge, part_succeq. apply partition_compatible. exact succeq'_sub.
-      unfold Ege, E_ge, part_succeq. apply partition_compatible. exact succeq'_sub.
+      apply compat_app.
+      unfold Rgt, R_gt, part_succ. apply partition_compat. exact succ'_sub.
+      unfold Egt, E_gt, part_succ. apply partition_compat. exact succ'_sub.
+      apply compat_app.
+      unfold Rge, R_ge, part_succeq. apply partition_compat. exact succeq'_sub.
+      unfold Ege, E_ge, part_succeq. apply partition_compat. exact succeq'_sub.
     Qed.
 
   End RelativeTerminationCriterion.
@@ -281,7 +292,8 @@ Module ExtendedMonotoneAlgebraResults (EMA : ExtendedMonotoneAlgebraType).
     Proof.
       intros. apply WF_incl with (red_mod nil R). apply red_incl_red_mod.
       apply ma_relative_termination. assumption. trivial.
-      simpl. apply WF_incl with (red (fst (partition part_succeq (snd (partition part_succ R))))).
+      simpl. apply WF_incl with
+      (red (fst (partition part_succeq (snd (partition part_succ R))))).
       apply red_mod_empty_incl_red. assumption.
     Qed.
 
@@ -289,8 +301,10 @@ Module ExtendedMonotoneAlgebraResults (EMA : ExtendedMonotoneAlgebraType).
 
   Ltac prove_termination :=  
     match goal with
-    | |- WF (red ?R) => apply ma_termination; simpl; trivial; try apply WF_empty
-    | |- WF (red_mod ?E ?R) => apply ma_relative_termination; simpl; trivial; try apply WF_mod_empty
+    | |- WF (red ?R) =>
+      apply ma_termination; simpl; trivial; try apply WF_empty
+    | |- WF (red_mod ?E ?R) =>
+      apply ma_relative_termination; simpl; trivial; try apply WF_mod_empty
     end.
 
 End ExtendedMonotoneAlgebraResults.
